Aux.ec
@@ -21,6 +21,16 @@ qed.
 
 
 
+lemma oip2b (a b c p : real) :  
+  (0%r < b) =>
+  (0%r <= p) =>
+      a = b * c - b * p \/  a = b * c + b * p
+   =>   `|a / b - c| = p.
+smt.
+qed.
+
+
+
 lemma oip3 (a b c eps : real) :  (0%r < b) => (0%r <= eps) =>
   `|a / b - c| <= eps => 
   exists (p : real),  0%r <= p <= eps  
@@ -29,3 +39,21 @@ lemma oip3 (a b c eps : real) :  (0%r < b) => (0%r <= eps) =>
 smt (oip1 oip2).
 qed.
 
+
+
+lemma oip4 (a c p : real) :  
+  (0%r <= p) =>
+   a = c - p \/  a = c + p
+   => `|a - c| = p.
+smt.
+qed.
+
+
+require import AllCore Distr FSet StdRing StdOrder StdBigop List.
+(*---*) import RField RealOrder Bigreal BRA.
+
+
+axiom big_geq0 p  : 0%r <= p <= 1%r => forall n, 
+ 0%r <= bigi predT (fun (i : int) => (1%r-p) ^ i * p) 0 n.
+axiom big_leq1 p  : 0%r <= p <= 1%r => forall n, 
+ bigi predT (fun (i : int) => (1%r-p) ^ i * p) 0 n <= 1%r.
